

A KINETIC REINTERPRETATION OF THERMODYNAMIC RESTRICTIONS OF CONTINUA

We aim to give a kinematic interpretation of the theory of thermodynamic continua developed by Prof. RAJAGOPAL and collaborators. Our starting point will be the BOLTZMANN EQUATION, i.e.

$$\underbrace{\partial_t f + \underline{v} \cdot \nabla_x f}_{\text{ADVECTION}} = \underbrace{Q[f, f]}_{\text{COLLISION}}$$

where $f(\underline{x}, \underline{v}, t)$ is the one-particle distribution function i.e. the probability density of finding one particle of an ensemble at the position $(\underline{x}, \underline{v})$ of the phase space at instant t . Furthermore the collision operator $Q[f, f]$ is defined as

$$Q[f, f] := \int_{\mathbb{R}^3} dv_* \underbrace{\int d\Omega d\psi B(\Omega, \psi, |\underline{v} - \underline{v}_*|)}_{\text{COLLISIONAL KERNEL}} [f(\underline{x}, \underline{v}', t) f(\underline{x}, \underline{v}'_*, t) - f(\underline{x}, \underline{v}, t) f(\underline{x}, \underline{v}_*, t)]$$

where \underline{v}' and \underline{v}'_* are the post collisional velocities, which we assume can be computed from \underline{v} and \underline{v}_* by means of a binary law, i.e.

$$\underline{v}' = \underline{v}'(\underline{v}, \underline{v}_*) \quad \underline{v}'_* = \underline{v}'_*(\underline{v}, \underline{v}_*)$$

For the moment being we will consider the BGK approximation of $Q[f, f]$, i.e.

$$Q[f, f] \approx \underbrace{\text{COLLISIONAL FREQUENCY}}_{\rightarrow} -\frac{1}{2} (f - f^{(0)})$$

where $f^{(0)}$ is the MAXWELLIAN DISTRIBUTION defined as,

$$f^{(0)}(\underline{x}, \underline{v}, t) = \frac{\rho(\underline{x}, t)}{(2\pi R\theta)^{3/2}} \exp\left(-\frac{|\underline{v} - \underline{u}(\underline{x}, t)|^2}{2R\theta}\right)$$

$$\stackrel{\text{EQUIPARTITION OF ENERGY THEOREM } e = \frac{3}{2} R\theta}{\uparrow} = \frac{\rho(\underline{x}, t)}{(\frac{4}{3}\pi e(\underline{x}, t))^{3/2}} \exp\left(-\frac{|\underline{v} - \underline{u}(\underline{x}, t)|^2}{\frac{4}{3}e}\right)$$

where $\rho(\underline{x}, t)$, $\underline{u}(\underline{x}, t)$ and $e(\underline{x}, t)$ are respectively the density, the macroscopic velocity and internal energy

defined as,

$$\rho(\underline{x}, t) = m n(\underline{x}, t) := m \int_{\mathbb{R}^d} f(\underline{x}, \underline{v}, t) d\underline{v}$$

$$\underline{u}(\underline{x}, t) = \frac{1}{n(\underline{x}, t)} \int_{\mathbb{R}^d} \underline{v} f(\underline{x}, \underline{v}, t) d\underline{v}$$

$$e(\underline{x}, t) = \frac{1}{n(\underline{x}, t)} \frac{1}{2} \int_{\mathbb{R}^d} \underline{w} \cdot \underline{w} f(\underline{x}, \underline{v}, t) d\underline{v}, \text{ with } \underline{w} := \underline{v} - \underline{u}.$$

Another macroscopic quantity that will be of prime importance even if not involved in the definition of $f^{(0)}$ is the ENTROPY, i.e.

$$\eta(\underline{x}, t) = \frac{1}{n(\underline{x}, t)} \int_{\mathbb{R}^d} f(\underline{x}, \underline{v}, t) \log[f(\underline{x}, \underline{v}, t)] d\underline{v}$$

Thus the BGK operator is constructed in such a way to conserve the density, linear momentum and energy of f . Furthermore as we will see later it is constructed to mimic another property of $Q[f, f]$, i.e. the relaxation to the Maxwellian $f^{(0)}$.

BALANCE LAWS

Testing the Boltzmann equation with the 3 (5 scalars) collision invariants, at the level of the binary interactions, we thus obtain:

$$\int_{\mathbb{R}^3} \psi(\underline{v}) Q[f, f] = \int_{\mathbb{R}} \psi(\underline{v}) Q_{BGK}[f, f] = 0 \quad \forall \psi \in \{m, m\underline{v}, \frac{1}{2}m|\underline{v}|^2\}.$$

This gives us 3 different balance laws, i.e.

$$\psi = m) \quad \partial_t \rho + \nabla_x \cdot (\rho \underline{u}) = 0 \quad \text{CONTINUITY EQUATION / BALANCE LAW OF MASS}$$

$$\psi = m\underline{v}) \quad \rho [\partial_t \underline{u} + (\nabla \underline{u}) \underline{u}] + \nabla_x \cdot \Pi = 0 \quad \text{BALANCE LAW OF LINEAR MOMENTUM}$$

where $\Pi(\underline{x}, t) = \int_{\mathbb{R}^3} m \underline{w} \otimes \underline{w} f(\underline{x}, \underline{v}, t)$ is the Cauchy stress tensor.

$$\Psi = \frac{1}{2} m |\underline{v}|^2 \quad \partial_t \left(\frac{1}{2} \rho |\underline{u}|^2 + \rho e \right) + \nabla_x \cdot \left(\frac{1}{2} \rho |\underline{u}|^2 \underline{u} + \rho e \underline{u} + \Pi \underline{u} + Q \right) = 0$$

This is the BALANCE LAW OF TOTAL ENERGY, where we have defined the HEAT FLUX VECTOR as,

$$Q(\underline{x}, t) := \int_{\mathbb{R}^3} \frac{1}{2} m |\underline{w}|^2 \underline{w} f(\underline{x}, \underline{v}, t) d\underline{v}.$$

This also implies the BALANCE LAW OF INTERNAL ENERGY, i.e.

$$\rho (\partial_t e + \nabla_x e \cdot \underline{u}) + \Pi : \nabla_x \underline{u} + \nabla_x \cdot Q = 0.$$

Similarly testing by $\Psi(\underline{x}, \underline{v}, t) = \log(f(\underline{x}, \underline{v}, t))$ we can obtain an evolution equation for the ENTROPY, i.e.

$$\rho (\partial_t \eta + \nabla_x \eta \cdot \underline{u}) + \nabla_x \cdot \Phi = \zeta (*) \text{ where}$$

$$\Phi(\underline{x}, t) = \int_{\mathbb{R}^3} m \log(f) f d\underline{v} \quad \text{ENTROPY FLUX}$$

$$\zeta(\underline{x}, t) = \int_{\mathbb{R}^3} \frac{1}{2} (f^{(0)} - f) \log(f) d\underline{v} \quad \text{ENTROPY PRODUCTION}$$

THERMODYNAMICS A key aspect of the Boltzmann equation is the so called Boltzmann inequality. Let us consider

$$\begin{aligned} \int d\underline{v} \frac{1}{2} (f^{(0)} - f) \log(f) d\underline{v} &= \int d\underline{v} \frac{1}{2} (f^{(0)} - f) \log(f^{(0)}) \\ &\quad - \int d\underline{v} \frac{1}{2} (f^{(0)} - f) \log(f^{(0)}) \\ &\quad + \underbrace{\int d\underline{v} \frac{1}{2} (f^{(0)} - f) \log(f^{(0)})}_{\text{VANISH}} \end{aligned}$$

$$= \int d\underline{v} \frac{1}{2} (f^{(0)} - f) (\log(f) - \log(f^{(0)})) \leq 0$$

This implies that the ENTROPY PRODUCTION is always NEGATIVE, which is a form of the second law of thermody. (3)

namics. We can also obtain another form of the II law of thermodynamics, introducing

$$H(t) := \int_{\Omega} \eta(x, t) dx \quad \text{where } \Omega \text{ is the volume occupied by the system of particles under consideration.}$$

Integrating (*) we thus get

$$\frac{dH}{dt} \leq \int_{\partial\Omega} \underline{n} \cdot \underline{\Phi}$$

This term vanishes when the system is thermodynamically isolated and thus we are left with the constant decrease of entropy $\frac{dH}{dt} \leq 0$.

In particular we observe that $\frac{dH}{dt} = 0 \Leftrightarrow f = f^{(0)}$ since obviously when $f = f^{(0)}$, $z = 0$. Suggesting that a system at thermodynamic isolation reaches equilibrium after enough time thus thermalising to a Maxwellian $f^{(0)}$.

Since we know that at thermodynamic equilibrium $f \searrow f^{(0)}$ we might think that near thermodynamic equilibrium f must be a perturbation around $f^{(0)}$.

This idea is formalised by the CHAPMAN-ENSKOG EXPANSION

where we assume that $f = \sum_{k=0}^{\infty} (k_n)^k f^{(k)}$ with

$$k_n := \frac{\lambda}{L} \quad \text{being the KNUDSEN NUMBER.}$$

λ ← MEAN FREE PATH
 L ← CHARACTERISTIC MACROSCOPIC LENGTH.

Using the relation between the thermal speed $v_T := \sqrt{2RT}$, the mean free path λ and the collision frequency one has

$$\boxed{\lambda = v_T z} \Rightarrow \boxed{k_n = \frac{v_T z}{L}} \Rightarrow \boxed{z = \frac{k_n L}{v_T}} \Rightarrow z \sim O\left(\frac{1}{k_n}\right). \quad (4)$$

ZEROTH - ORDER CHAPMAN - ENSKOG

We begin assuming that we are sufficiently close to the equilibrium that $f \approx f^{(0)}$. Thus we proceed deriving an equation of state, i.e.

$$\rho \eta^{(0)} = \int dv \log(f^{(0)}) f^{(0)} = \frac{3}{2} \log\left(\frac{2}{3} e(x,t) \rho(x,t)^{2/3}\right) \rho$$

thus implying that, $\eta^{(0)}(x,t) = \frac{3}{2} \log\left(\frac{2}{3} e(x,t) \rho(x,t)^{2/3}\right)$ and also by inverting this relation that,

$$\textcircled{1} \quad e^{(0)}(x,t) = \frac{3}{2} \exp\left(\frac{2}{3} \eta^{(0)}(x,t)\right) \rho(x,t)^{2/3} = e^{(0)}(\eta, \rho).$$

We now use the BALANCE LAW OF INTERNAL ENERGY, and the one for the ENTROPY to obtain the following:

$$\frac{d}{dt} e = \frac{\partial e}{\partial \rho} \frac{d\rho}{dt} + \frac{\partial e}{\partial \eta} \frac{d\eta}{dt} \quad \begin{array}{l} \text{By the thermodynamic definition} \\ \text{of temperature } \frac{\partial e}{\partial \eta} = \theta \end{array}$$

$$\begin{array}{l} \text{By the thermodynamic definition of pressure,} \\ \hat{p} = \rho^2 \frac{\partial e}{\partial \eta} \end{array} \quad \begin{array}{l} \text{By the balance law of internal energy} \\ \frac{d}{dt} e = \theta \nabla_x \cdot u \end{array}$$

$$\text{thus we have that, } \frac{d\eta}{dt} = \frac{1}{\theta} \left[\frac{de}{dt} - \hat{p}/\rho^2 \frac{d\rho}{dt} \right].$$

$$\text{Hence we have, } \frac{d\eta}{dt} = \frac{1}{\theta} \left[-\frac{1}{\rho} (\pi : \nabla_x u + \nabla_x \cdot Q) + \hat{p}/\rho \nabla_x \cdot u \right]$$

$$\rho \frac{d\eta^{(0)}}{dt} = \frac{1}{\theta} \left[\hat{p} (\nabla_x \cdot u) - \pi : \nabla_x u - \nabla_x \cdot Q \right]$$

$$\text{" } \nabla_x \cdot \Phi^{(0)} - \dot{z}^{(0)} \Rightarrow \theta (\nabla_x \cdot \Phi - \dot{z}) = [\hat{p} (\nabla_x \cdot u) - \pi : \nabla_x u - \nabla_x \cdot Q]$$

We now compute $\dot{z}^{(0)}$ and $\Phi^{(0)}$, notice that $\dot{z}^{(0)}$ is trivially zero and that we can compute

$$\Phi^{(0)}(x,t) = \int \underline{w} \log(f^{(0)}) f^{(0)} d\underline{w}$$

$$\searrow \log(n(x,t)) + \log(c(x,t)) - \frac{|\underline{w}|^2}{2\kappa} \frac{3}{4} e^{-1}$$

$$\Phi^{(0)}(x,t) = \underbrace{\int \underline{w} \log(n(x,t)) f^{(0)} d\underline{w}}_0 + \underbrace{\int \underline{w} \log(c(x,t)) f^{(0)} d\underline{w}}_0$$

$$+ \int \underline{w} \frac{|\underline{w}|^2}{2\kappa} \frac{3}{4} e^{-1} f^{(0)} d\underline{w} = Q_{4/3} e$$

Notice now that $Q^{(0)} = \int \underline{w} |\underline{w}|^2 d\underline{w} = 0$ because the skewness of a Gaussian is zero. Thus we are left with the constraint,

$$\hat{p}(\nabla \cdot u) - \Pi : \nabla_x u = 0$$

$$\underline{\underline{I}} \hat{p} = \underline{\underline{\Pi}}, \text{ since this must be valid } \forall u.$$

REMARK

FIRST ORDER CHAPMAN-ENSKOG

We will now assume that the K_n is sufficiently small that we can write the truncated CHAPMAN-ENSKOG EXPANSION

$$f = f^{(0)} + (K_n) f^{(1)}.$$

We thus introduce multiple time variables, i.e. $t_0 = t$
 $t_1 = K_n t$ and treat f as a function of each time scale, i.e. $f = f(x, v, t_0, t_1)$ and thus expanding the BOLTZMANN EQUATION we obtain,

$$(\partial_{t_0} + K_n \partial_{t_1}) (f^{(0)} + K_n f^{(1)}) + v \cdot \nabla_x (f^{(0)} + K_n f^{(1)}) = \frac{1}{2} f^{(1)} \quad (*)$$

where we have rescaled the collisional frequency by K_n . For this expansion to be unique we need to ask that the following solvability conditions are satisfied,

$$\int dv f^{(1)} = 0, \quad \int dv \underline{w} f^{(1)} = 0, \quad \int dv \frac{1}{2} |\underline{w}|^2 f^{(1)} = 0.$$

Collecting the zero-th order term in K_n in (*) we obtain,

$$f^{(1)} = (\partial_{t_0} f^{(0)} + v \cdot \nabla_x f^{(0)}).$$

Which we can compute explicitly to be,

$$f_{Bek}^{(1)} = - \hat{z} f^{(0)} \left[\frac{m}{\frac{2}{3}e} (\underline{w} \otimes \underline{w}) : \mathbb{S} + \left(\frac{m \underline{w} \cdot \underline{w}}{2/3 e} - \frac{5}{2} \right) \underline{w} \cdot \frac{\nabla e}{e} \right]$$

$$\text{where } \mathbb{S} = \frac{1}{2} (\nabla u + \nabla u^T) - \frac{1}{3} (\nabla \cdot u) \underline{\underline{I}}.$$

Notice that we now want to compute an equation of state similarly to before and we do so as follows,

We notice that $\log(1+x) = x + O(x^2)$ thus if $x = K_n \frac{f^{(1)}}{f^{(0)}}$ we have that $K_n \ll 1$ implies $\log\left(\frac{f^{(0)} + K_n f^{(1)}}{f^{(0)}}\right) = K_n \frac{f^{(1)}}{f^{(0)}}$ and thus $\log(f^{(0)} + K_n f^{(1)}) = K_n f^{(1)} / f^{(0)} + \log(f^{(0)})$.

(7)

Thus we can write,

$$\begin{aligned}
 p \eta^{(1)} &= \int (f^{(0)} + k_n f^{(1)}) \log (f^{(0)} + k_n f^{(1)}) dv \\
 &= \int (f^{(0)} + k_n f^{(1)}) (\log (f^{(0)}) + k_n f^{(1)} / f^{(0)}) dv \\
 &= \eta^{(0)} + k_n \int f^{(1)} (\log (f^{(0)}) + 1) + \mathcal{O}(k_n^2) \\
 &= \eta^{(0)} + \mathcal{O}(k_n^2). \quad \leftarrow \text{VANISH BY SOLVABILITY CONDITION.} \\
 &= \frac{3}{2} \log \left(\frac{2}{3} e(x,t) f(x,t)^{-2/3} \right) \Rightarrow \textcircled{\text{X}} e = e(\eta, \rho).
 \end{aligned}$$

$$\begin{aligned}
 \Phi^{(1)} &= \int w \log (f^{(0)} + k_n f^{(1)}) (f^{(0)} + k_n f^{(1)}) dv \\
 &= \underbrace{\Phi^{(0)}_0 + k_n \int w \log (f^{(0)}) f^{(1)} dv}_{Q^{(1)} / \frac{4}{3} e} + \mathcal{O}(k_n^2)
 \end{aligned}$$

Lastly we notice that,

$$\begin{aligned}
 z^{(1)} &= \int dv \log (f^{(0)} + k_n f^{(1)}) \frac{1}{2} (f^{(0)} - f^{(0)} - k_n f^{(1)}) \\
 &= -\frac{k_n}{2} \int dv [\log (f^{(0)}) + k_n f^{(1)} / f^{(0)}] f^{(1)} \\
 &= -\frac{k_n^2}{2} \int dv f^{(1)} \cdot f^{(1)} / f^{(0)} = 2\nu \mathbb{S} : \mathbb{S} + \sum_k^{\text{K}=\text{K}(e)} \frac{\nabla e \cdot \nabla e}{e}
 \end{aligned}$$

Thus we are left with the fact that $k_n \searrow 0$ is equivalent to maximising $|z|$ subject to $2\nu \mathbb{S} : \mathbb{S} + k \frac{\nabla e \cdot \nabla e}{e} = -\nabla u : \Pi + \hat{p} \nabla \cdot u$
 hence $\hat{p} = \frac{1}{2} \text{tr}(\nabla u)$, $\text{dev}(\sigma) = \mathbb{S}$ and $Q = k \nabla e$.